examples/mutsum/MutHeader.v
@@ -25,11 +25,10 @@ Section PROOF.
 
   Context `{Σ: GRA.t}.
 
-  Definition GlobalStb: list (gname * fspec) := [
-    ("main", mk "F" (X:=unit) (fun _ varg_high varg_low _ => varg_high = varg_low) (fun _ vret_high vret_low _ => vret_high = vret_low) (fun _ => None));
-    ("f", mk "F" (X:=nat) (fun n _ varg _ => varg = [Vint (Z.of_nat n)]↑) (fun n _ vret _ => vret = (Vint (Z.of_nat (sum n)))↑) (fun _ => None)) ;
-    ("g", mk "F" (X:=nat) (fun n _ varg _ => varg = [Vint (Z.of_nat n)]↑) (fun n _ vret _ => vret = (Vint (Z.of_nat (sum n)))↑) (fun _ => None))
-  ].
+  Definition main_spec: fspec := mk_simple "F" (X:=unit) top3 top3 (fun _ => ord_top).
+  Definition f_spec:    fspec := mk_simple "F" (X:=nat) (fun n varg _ => varg = [Vint (Z.of_nat n)]↑) (fun n vret _ => vret = (Vint (Z.of_nat (sum n)))↑) (fun _ => ord_top).
+  Definition g_spec:    fspec := mk_simple "G" (X:=nat) (fun n varg _ => varg = [Vint (Z.of_nat n)]↑) (fun n vret _ => vret = (Vint (Z.of_nat (sum n)))↑) (fun _ => ord_top).
+  Definition GlobalStb: list (gname * fspec) := [("main", main_spec); ("f", f_spec); ("g", g_spec)].
 
 End PROOF.
 
